[sledge sem] Fix global variables
Summary:
Add a field to LLAIR variables to indicate whether they are global or
local. Update the LLVM semantics for constant expression evaluation to
be relational, so that it doesn't have to have an answer for references
to undefined globals.

Reviewed By: jberdine

Differential Revision: D19446312

fbshipit-source-id: 9bbfd180e

sledge/semantics/llairScript.sml
@@ -54,7 +54,8 @@ End
 (* Based on the constructor functions in exp.mli rather than the type definition *)
 Datatype:
   exp =
-  | Var var
+  (* Args: variable name, true for globals *)
+  | Var var bool
   | Nondet
   (* Args: function name, block name *)
   | Label label
@@ -262,7 +263,12 @@ Inductive eval_exp:
   (∀s v r.
    flookup s.locals v = Some r
    ⇒
-   eval_exp s (Var v) r) ∧
+   eval_exp s (Var v F) r) ∧
+
+  (∀s v r.
+   flookup s.glob_addrs v = Some r
+   ⇒
+   eval_exp s (Var v T) (FlatV (n2i r pointer_size))) ∧
 
   (* TODO: Nondet I guess we need to know the type here *)
   (* TODO: Label *)
